Picinae_i386.v
@@ -16,12 +16,12 @@
    To compile this module, first load and compile:       MMMMMMMMMMMMMM7..$MNDM+
    * Picinae_core                                         MMDMMMMMMMMMZ7..$DM$77
    * Picinae_theory                                        MMMMMMM+MMMZ7..7ZM~++
-   * Picinae_finterp                                        MMMMMMMMMMM7..ZNOOMZ
-   * Picinae_statics                                         MMMMMMMMMM$.$MOMO=7
-   * Picinae_slogic                                           MDMMMMMMMO.7MDM7M+
-   Then compile this module with menu option                   ZMMMMMMMM.$MM8$MN
-   Compile->Compile_buffer.                                    $ZMMMMMMZ..MMMOMZ
-                                                                ?MMMMMM7..MNN7$M
+   * Picinae_statics                                        MMMMMMMMMMM7..ZNOOMZ
+   * Picinae_finterp                                         MMMMMMMMMM$.$MOMO=7
+   * Picinae_simplifier_*                                     MDMMMMMMMO.7MDM7M+
+   * Picinae_ISA                                               ZMMMMMMMM.$MM8$MN
+   Then compile this module with menu option                   $ZMMMMMMZ..MMMOMZ
+   Compile->Compile_buffer.                                     ?MMMMMM7..MNN7$M
                                                                  ?MMMMMZ..MZM$ZZ
                                                                   ?$MMMZ7.ZZM7DZ
                                                                     7MMM$.7MDOD7
@@ -37,7 +37,7 @@ Require Export Picinae_theory.
 Require Export Picinae_statics.
 Require Export Picinae_finterp.
 Require Export Picinae_simplifier_v1_1.
-(* Require Export Picinae_slogic. *)
+Require Export Picinae_ISA.
 Require Import NArith.
 Require Import Program.Equality.
 Require Import Structures.Equalities.
@@ -45,33 +45,52 @@ Open Scope N.
 
 (* Variables found in IL code lifted from x86 native code: *)
 Inductive x86var :=
-  (* Main memory: MemT 32 *)
+  (* Main memory: *)
   | V_MEM32
   (* Flags (1-bit registers): *)
-  | R_AF | R_CF | R_DF | R_OF | R_PF | R_SF | R_ZF (* NumT 1 *)
+  | R_AF | R_CF | R_DF | R_OF | R_PF | R_SF | R_ZF
   (* Segment selectors (16-bit registers): *)
-  | R_CS | R_DS | R_ES | R_FS | R_GS | R_SS (* NumT 16 *)
+  | R_CS | R_DS | R_ES | R_FS | R_GS | R_SS
   (* Floating point control register (16-bit): *)
-  | R_FPU_CONTROL (* NumT 16 *)
+  | R_FPU_CONTROL
   (* Floating point registers (80-bit): *)
-  | R_ST0 | R_ST1 | R_ST2 | R_ST3 | R_ST4 | R_ST5 | R_ST6 | R_ST7 (* NumT 80 *)
+  | R_ST0 | R_ST1 | R_ST2 | R_ST3 | R_ST4 | R_ST5 | R_ST6 | R_ST7
   (* General-purpose registers (32-bit): *)
-  | R_EAX | R_EBX | R_ECX | R_EDX | R_EDI | R_ESI (* NumT 32 *)
+  | R_EAX | R_EBX | R_ECX | R_EDX | R_EDI | R_ESI
   (* Stack pointer and base pointer (32-bit): *)
-  | R_ESP | R_EBP (* NumT 32 *)
+  | R_ESP | R_EBP
   (* Modifiable segment base registers (32-bit): *)
-  | R_FS_BASE | R_GS_BASE (* NumT 32 *)
+  | R_FS_BASE | R_GS_BASE
   (* Descriptor table registers (32-bit): *)
-  | R_LDTR | R_GDTR (* NumT 32 *)
+  | R_LDTR | R_GDTR
   (* SSE control register (32-bit): *)
-  | R_MXCSR (* NumT 32 *)
+  | R_MXCSR
   (* MMX and SSE registers (256-bit): *)
   | R_YMM0 | R_YMM1 | R_YMM2  | R_YMM3  | R_YMM4  | R_YMM5  | R_YMM6  | R_YMM7
   | R_YMM8 | R_YMM9 | R_YMM10 | R_YMM11 | R_YMM12 | R_YMM13 | R_YMM14 | R_YMM15
   (* These meta-variables model page access permissions: *)
   | A_READ | A_WRITE
-  (* Temporaries introduced by the BIL lifter: *)
+  (* Temporaries introduced by the lifter: *)
   | V_TEMP (n:N).
+
+(* Declare the types (i.e., bitwidths) of all the CPU registers: *)
+Definition x86typctx v :=
+  match v with
+  | V_MEM32 => Some (8*2^32)
+  | R_AF | R_CF | R_DF | R_OF | R_PF | R_SF | R_ZF => Some 1
+  | R_CS | R_DS | R_ES | R_FS | R_GS | R_SS => Some 16
+  | R_FPU_CONTROL => Some 16
+  | R_ST0 | R_ST1 | R_ST2 | R_ST3 | R_ST4 | R_ST5 | R_ST6 | R_ST7 => Some 80
+  | R_EAX | R_EBX | R_ECX | R_EDX | R_EDI | R_ESI => Some 32
+  | R_ESP | R_EBP => Some 32
+  | R_FS_BASE | R_GS_BASE => Some 32
+  | R_LDTR | R_GDTR => Some 32
+  | R_MXCSR => Some 32
+  | R_YMM0 | R_YMM1 | R_YMM2  | R_YMM3  | R_YMM4  | R_YMM5  | R_YMM6  | R_YMM7
+  | R_YMM8 | R_YMM9 | R_YMM10 | R_YMM11 | R_YMM12 | R_YMM13 | R_YMM14 | R_YMM15 => Some 256
+  | A_READ | A_WRITE => Some (2^32)
+  | V_TEMP _ => None
+  end.
 
 (* Create a UsualDecidableType module (which is an instance of Typ) to give as
    input to the Architecture module, so that it understands how the variable
@@ -89,11 +108,12 @@ End MiniX86VarEq.
 Module X86Arch <: Architecture.
   Module Var := Make_UDT MiniX86VarEq.
   Definition var := Var.t.
-  Definition store := var -> value.
+  Definition store := var -> N.
+  Definition typctx := var -> option bitwidth.
+  Definition archtyps := x86typctx.
 
-  Definition mem_bits := 8%positive.
-  Definition mem_readable s a := exists r, s A_READ = VaM r 32 /\ r a <> 0.
-  Definition mem_writable s a := exists w, s A_WRITE = VaM w 32 /\ w a <> 0.
+  Definition mem_readable s a := N.testbit (s A_READ) a = true.
+  Definition mem_writable s a := N.testbit (s A_WRITE) a = true.
 End X86Arch.
 
 (* Instantiate the Picinae modules with the x86 identifiers above. *)
@@ -105,72 +125,26 @@ Module Statics_i386 := PicinaeStatics IL_i386 Theory_i386.
 Export Statics_i386.
 Module FInterp_i386 := PicinaeFInterp IL_i386 Theory_i386 Statics_i386.
 Export FInterp_i386.
-(* Module SLogic_i386 := PicinaeSLogic IL_i386.
-Export SLogic_i386. *)
-
-Module PSimpl_i386 := Picinae_Simplifier_Base.
+Module PSimpl_i386 := Picinae_Simplifier_Base IL_i386.
 Export PSimpl_i386.
 Module PSimpl_i386_v1_1 := Picinae_Simplifier_v1_1 IL_i386 Theory_i386 Statics_i386 FInterp_i386.
 Ltac PSimplifier ::= PSimpl_i386_v1_1.PSimplifier.
 
-(* Introduce unique aliases for tactics in case user loads multiple architectures. *)
-Tactic Notation "i386_psimpl" uconstr(e) "in" hyp(H) := psimpl_exp_hyp uconstr:(e) H.
-Tactic Notation "i386_psimpl" uconstr(e) := psimpl_exp_goal uconstr:(e).
-Tactic Notation "i386_psimpl" "in" hyp(H) := psimpl_all_hyp H.
-Tactic Notation "i386_psimpl" := psimpl_all_goal.
-
-(* To use a different simplifier version (e.g., v1_0) put the following atop
-   your proof .v file:
+(* To use a different simplifier version (e.g., v1_0) put the following atop your proof .v file:
 Require Import Picinae_simplifier_v1_0.
-Module PSimpl_i386_v1_0 := Picinae_Simplifier_v1_0 IL_i386 Statics_i386 FInterp_i386.
+Module PSimpl_i386_v1_0 := Picinae_Simplifier_v1_0 IL_i386 Theory_i386 Statics_i386 FInterp_i386.
 Ltac PSimplifier ::= PSimpl_i386_v1_0.PSimplifier.
 *)
 
-(* Declare the types (i.e., bitwidths) of all the CPU registers: *)
-Definition x86typctx v :=
-  match v with
-  | V_MEM32 => Some (MemT 32)
-  | R_AF | R_CF | R_DF | R_OF | R_PF | R_SF | R_ZF => Some (NumT 1)
-  | R_CS | R_DS | R_ES | R_FS | R_GS | R_SS => Some (NumT 16)
-  | R_FPU_CONTROL => Some (NumT 16)
-  | R_ST0 | R_ST1 | R_ST2 | R_ST3 | R_ST4 | R_ST5 | R_ST6 | R_ST7 => Some (NumT 80)
-  | R_EAX | R_EBX | R_ECX | R_EDX | R_EDI | R_ESI => Some (NumT 32)
-  | R_ESP | R_EBP => Some (NumT 32)
-  | R_FS_BASE | R_GS_BASE => Some (NumT 32)
-  | R_LDTR | R_GDTR => Some (NumT 32)
-  | R_MXCSR => Some (NumT 32)
-  | R_YMM0 | R_YMM1 | R_YMM2  | R_YMM3  | R_YMM4  | R_YMM5  | R_YMM6  | R_YMM7
-  | R_YMM8 | R_YMM9 | R_YMM10 | R_YMM11 | R_YMM12 | R_YMM13 | R_YMM14 | R_YMM15 => Some (NumT 256)
-  | A_READ | A_WRITE => Some (MemT 32)
-  | V_TEMP _ => None
-  end.
+Module ISA_i386 := Picinae_ISA IL_i386 PSimpl_i386 Theory_i386 Statics_i386 FInterp_i386.
+Export ISA_i386.
 
-Definition x86_wtm {s v m w} := @models_wtm v x86typctx s m w.
-Definition x86_regsize {s v n w} := @models_regsize v x86typctx s n w.
-
-
-
-(* Create some automated machinery for simplifying symbolic expressions commonly
-   arising from x86 instruction operations.  Mostly this involves simplifying
-   (e mod 2^w) whenever e < 2^w. *)
-
-(* Define an abbreviation for x86's parity flag computation, which produces
-   uncomfortably large symbolic expressions. *)
-Definition parity n :=
-  N.lnot ((N.lxor
-    (N.shiftr (N.lxor (N.shiftr (N.lxor (N.shiftr n 4) n) 2)
-                      (N.lxor (N.shiftr n 4) n)) 1)
-    (N.lxor (N.shiftr (N.lxor (N.shiftr n 4) n) 2)
-            (N.lxor (N.shiftr n 4) n))) mod 2^1) 1.
-
-Lemma fold_parity: forall n,
-  N.lnot ((N.lxor
-    (N.shiftr (N.lxor (N.shiftr (N.lxor (N.shiftr n 4) n) 2)
-                      (N.lxor (N.shiftr n 4) n)) 1)
-    (N.lxor (N.shiftr (N.lxor (N.shiftr n 4) n) 2)
-            (N.lxor (N.shiftr n 4) n))) mod 2^1) 1
-  = parity n.
-Proof. intro. reflexivity. Qed.
+(* Introduce unique aliases for tactics in case user loads multiple architectures. *)
+Tactic Notation "i386_psimpl" uconstr(e) "in" hyp(H) := psimpl_exp_hyp uconstr:(e) H.
+Tactic Notation "i386_psimpl" uconstr(e) := psimpl_exp_goal uconstr:(e).
+Tactic Notation "i386_psimpl" "in" hyp(H) := psimpl_hyp H.
+Tactic Notation "i386_psimpl" := psimpl_goal.
+Ltac x86_step := ISA_step.
 
 
 (* Simplify memory access propositions by observing that on x86, the only part
@@ -209,28 +183,8 @@ Proof.
   intros. unfold MemAcc, mem_writable. rewrite !update_updated. reflexivity.
 Qed.
 
-
-(* getmem assembles bytes into words by logical-or'ing them together, but
-   sometimes it is easier to reason about them as if they were summed.  The
-   following theorem proves that logical-or and addition are the same when
-   the operands share no common bits. *)
-Theorem lor_plus:
-  forall a b (A0: N.land a b = 0), N.lor a b = a + b.
-Proof.
-  intros. rewrite <- N.lxor_lor, N.add_nocarry_lxor by assumption. reflexivity.
-Qed.
-
-(* (a & b) ^ c = (a ^ c) & b whenever b & c = c *)
-Lemma lxor_land:
-  forall a b c, N.land b c = c -> N.lxor (N.land a b) c = N.land (N.lxor a c) b.
-Proof.
-  intros. apply N.bits_inj. apply N.bits_inj_iff in H. intro n. specialize (H n).
-  do 2 rewrite N.land_spec, N.lxor_spec. rewrite <- H, N.land_spec.
-  repeat destruct (N.testbit _ n); reflexivity.
-Qed.
-
 (* Simplify x86 memory access assertions produced by step_stmt. *)
-Ltac simpl_memaccs H :=
+Ltac simpl_memaccs H ::=
   try lazymatch type of H with context [ MemAcc mem_writable ] =>
     rewrite ?memacc_write_frame, ?memacc_write_updated in H by discriminate 1
   end;
@@ -238,196 +192,16 @@ Ltac simpl_memaccs H :=
     rewrite ?memacc_read_frame, ?memacc_read_updated in H by discriminate 1
   end.
 
-(* The user can ignore all assigned values to specified variables by
-   redefining x86_ignore.  Example:
-     Ltac x86_ignore v ::= constr:(match v with R_EAX => true | _ => false end).
- *)
-Ltac x86_ignore v := constr:(false).
-Ltac x86_abstract_vars H :=
-  repeat match type of H with context [ update ?s ?v ?u ] =>
-    let b := ltac:(x86_ignore v) in
-    lazymatch eval cbv in b with true =>
-      lazymatch u with
-      | VaN ?n ?w =>
-          tryif is_var n then fail else
-          let tmp := fresh "n" in
-          pose (tmp := n);
-          change (update s v (VaN n w)) with (update s v (VaN tmp w)) in H;
-          clearbody tmp
-      | VaM ?m ?w =>
-          tryif is_var m then fail else
-          let tmp := fresh "m" in
-          pose (tmp := m);
-          change (update s v (VaM m w)) with (update s v (VaM tmp w)) in H;
-          clearbody tmp
-      end
-    | _ => fail
-    end
-  end.
-
-Ltac generalize_trace :=
-  lazymatch goal with
-  | [ |- nextinv ?p ?Invs ?xp ?b (?xs'::?xs1::?t1++?xs0::?t) ] =>
-    change (nextinv p Invs xp b (xs'::(xs1::t1)++(xs0::t)));
-    let t' := fresh t1 in generalize (xs1::t1); intro t'; clear t1; rename t' into t1
-  | [ |- nextinv ?p ?Invs ?xp ?b (?xs'::?xs1::?xs0::?t) ] =>
-    change (nextinv p Invs xp b (xs'::(xs1::nil)++(xs0::t)));
-    let t' := fresh "t" in generalize (xs1::nil); intro t'
-  end.
-
-(* Syntax: generalize_frame m as x
-   Result: Find any goal expressions of the form m[a1:=u1]...[an:=un] where
-   a1..an are adjacent memory addresses, and compact them to expressions
-   of the form m[a:=x], where a=max(a1,...,an) and x is a user-specified name.
-   This is useful for abstracting a series of pushes that form a callee's
-   local stack frame into a single write of the entire byte array. *)
-Ltac generalize_frame_forward bytes w en m len1 a1 u1 len2 a2 u2 :=
-  let x := fresh in let H := fresh in let H' := fresh in
-  evar (x:N);
-  eassert (H: setmem w en len2 (setmem w en len1 m a1 u1) a2 u2 = setmem w en _ m a2 x);
-  [ subst x; eenough (H':_);
-    [ transitivity (setmem w en len2 (setmem w en len1 m a1 u1) (msub w a1 len2) u2);
-      [ apply f_equal2; [ exact H' | reflexivity ]
-      | etransitivity;
-        [ etransitivity;
-          [ apply setmem_merge_rev; reflexivity
-          | apply f_equal4; [psimpl|..]; reflexivity ]
-        | apply f_equal2; [ symmetry; exact H' | reflexivity ] ] ]
-    | psimpl; reflexivity ]
-  | rewrite H; clear H; clearbody x; try clear u1; try clear u2;
-    rename x into bytes ].
-Ltac generalize_frame_backward bytes w en m len1 a1 u1 len2 a2 u2 :=
-  let x := fresh in let H := fresh in let H' := fresh in
-  evar (x:N);
-  eassert (H: setmem w en len2 (setmem w en len1 m a1 u1) a2 u2 = setmem w en _ m a1 x);
-  [ subst x; eenough (H':_);
-    [ transitivity (setmem w en len2 (setmem w en len1 m a1 u1) ((a1+len1) mod 2^w) u2);
-      [ apply f_equal2; [ exact H' | reflexivity ]
-      | rewrite setmem_mod_l; etransitivity;
-        [ etransitivity;
-          [ apply setmem_merge; reflexivity
-          | apply f_equal4; [psimpl|..]; reflexivity ]
-        | apply f_equal2; reflexivity ] ]
-    | psimpl; try reflexivity ]
-  | rewrite H; clear H; clearbody x; try clear u1; try clear u2;
-    rename x into bytes ].
-Ltac generalize_frame m bytes :=
-  match goal with |- context [ setmem ?w ?en ?len2 (setmem ?w ?en ?len1 m ?a1 ?u1) ?a2 ?u2 ] =>
-    first [ generalize_frame_forward bytes w en m len1 a1 u1 len2 a2 u2
-          | generalize_frame_backward bytes w en m len1 a1 u1 len2 a2 u2 ]
-  end.
-Tactic Notation "generalize_frame" constr(m) "as" ident(bytes) :=
-  generalize_frame m bytes; repeat generalize_frame m bytes.
-
-(* Values of IL temp variables are ignored by the x86 interpreter once the IL
-   block that generated them completes.  We can therefore generalize them
-   away at IL block boundaries to simplify the expression. *)
-Ltac generalize_temps H :=
-  repeat match type of H with context [ update ?s (V_TEMP ?n) ?u ] =>
-    tryif is_var u then fail else
-    lazymatch type of H with context [ Var (V_TEMP n) ] => fail | _ =>
-      let tmp := fresh "tmp" in
-      pose (tmp := u);
-      change (update s (V_TEMP n) u) with (update s (V_TEMP n) tmp) in H;
-      clearbody tmp;
-      try fold value in tmp
-    end
-  end.
-
-(* Symbolically evaluate an x86 machine instruction for one step, and simplify
-   the resulting Coq expressions. *)
-Ltac x86_step_and_simplify XS :=
-  step_stmt XS;
-  x86_abstract_vars XS;
-  psimpl_vals_hyp XS;
-  simpl_memaccs XS;
-  destruct_memaccs XS;
-  generalize_temps XS.
-
-(* Introduce automated machinery for verifying an x86 machine code subroutine
-   (or collection of subroutines) by (1) defining a set of Floyd-Hoare
-   invariants (including pre- and post-conditions) and (2) proving that
-   symbolically executing the program starting at any invariant point in a
-   state that satisfies the program until the next invariant point always
-   yields a state that satisfies the reached invariant.  This proves partial
-   correctness of the subroutine.
-
-   In order for this methodology to prove that a post-condition holds at
-   subroutine exit, we must attach one of these invariants (the post-condition)
-   to the return address of the subroutine.  This is a somewhat delicate
-   process, since unlike most other code addresses, the exact value of the
-   return address is an unknown (defined by the caller).  We therefore adopt
-   the convention that subroutines "exit" whenever control flows to an address
-   for which no IL code is defined at that address.  This allows proving
-   correctness of a subroutine by lifting only the subroutine to IL code (or
-   using the pmono theorems from Picinae_theory to isolate only the subroutine
-   from a larger program), leaving the non-subroutine code undefined (None). *)
-
-
-(* Some versions of Coq check injection-heavy proofs very slowly (at Qed).
-   This slow-down can be avoided by sequestering prevalent injections into
-   lemmas, as we do here. *)
-Remark inj_prog_stmt: forall (sz1 sz2: N) (q1 q2: stmt),
-                      Some (sz1,q1) = Some (sz2,q2) -> sz1=sz2 /\ q1=q2.
-Proof. injection 1 as. split; assumption. Qed.
-
-(* Simplify (exitof a x) without expanding a. *)
-Remark exitof_none a: exitof a None = Addr a. Proof eq_refl.
-Remark exitof_some a x: exitof a (Some x) = x. Proof eq_refl.
-
-(* If asked to step the computation when we're already at an invariant point,
-   just make the proof goal be the invariant. *)
-Ltac x86_invhere :=
-  eapply nextinv_here; [ reflexivity | hnf; psimpl_vals_goal ].
-
-(* If we're not at an invariant, symbolically interpret the program for one
-   machine language instruction.  (The user can use "do" to step through many
-   instructions, but often it is wiser to pause and do some manual
-   simplification of the state at various points.) *)
-Ltac x86_invseek :=
-  eapply NIStep; [reflexivity|reflexivity|];
-  let s := fresh "s" in let x := fresh "x" in let XS := fresh "XS" in
-  intros s x XS;
-  x86_step_and_simplify XS;
-  repeat lazymatch type of XS with
-         | s=_ /\ x=_ => destruct XS; subst s x
-         | exec_stmt _ (if ?c then _ else _) _ _ =>
-             let BC := fresh "BC" in destruct c eqn:BC;
-             x86_step_and_simplify XS
-         | exec_stmt _ (N.iter _ _ _) _ _ => fail
-         | _ => x86_step_and_simplify XS
-         end;
-  try generalize_trace;
-  repeat match goal with [ u:value |- _ ] => clear u
-                       | [ n:N |- _ ] => clear n
-                       | [ m:addr->N |- _ ] => clear m end;
-  try lazymatch goal with |- context [ exitof (N.add ?m ?n) ] => simpl (N.add m n) end;
-  try first [ rewrite exitof_none | rewrite exitof_some ].
-
-(* Clear any stale memory-access hypotheses (arising from previous computation
-   steps) and either step to the next machine instruction (if we're not at an
-   invariant) or produce an invariant as a proof goal. *)
-Ltac x86_step :=
-  repeat match goal with [ H: MemAcc _ _ _ _ _ |- _ ] => clear H end;
-  first [ x86_invseek; try x86_invhere | x86_invhere ].
-
+(* Define ISA-specific notations: *)
 
 Declare Scope i386_scope.
 Delimit Scope i386_scope with i386.
-Bind Scope i386_scope with stmt exp typ trace.
+Bind Scope i386_scope with stmt exp trace.
 Open Scope i386_scope.
 Notation " s1 $; s2 " := (Seq s1 s2) (at level 75, right associativity) : i386_scope.
 
 Module X86Notations.
 
-Notation "Ⓜ m" := (VaM m 32) (at level 20, format "'Ⓜ' m") : i386_scope. (* memory value *)
-Notation "ⓑ u" := (VaN u 1) (at level 20, format "'ⓑ' u"). (* bit value *)
-Notation "Ⓑ u" := (VaN u 8) (at level 20, format "'Ⓑ' u"). (* byte value *)
-Notation "Ⓦ u" := (VaN u 16) (at level 20, format "'Ⓦ' u"). (* word value *)
-Notation "Ⓓ u" := (VaN u 32) (at level 20, format "'Ⓓ' u"). (* dword value *)
-Notation "Ⓠ u" := (VaN u 64) (at level 20, format "'Ⓠ' u"). (* quad word value *)
-Notation "Ⓧ u" := (VaN u 128) (at level 20, format "'Ⓧ' u"). (* xmm value *)
-Notation "Ⓨ u" := (VaN u 256) (at level 20, format "'Ⓨ' u"). (* ymm value *)
 Notation "m Ⓑ[ a  ]" := (getmem 32 LittleE 1 m a) (at level 30) : i386_scope. (* read byte from memory *)
 Notation "m Ⓦ[ a  ]" := (getmem 32 LittleE 2 m a) (at level 30) : i386_scope. (* read word from memory *)
 Notation "m Ⓓ[ a  ]" := (getmem 32 LittleE 4 m a) (at level 30) : i386_scope. (* read dword from memory *)
