Picinae_simplifier_base.v
@@ -1,6 +1,6 @@
 (* Picinae: Platform In Coq for INstruction Analysis of Executables       ZZM7DZ
                                                                           $MNDM7
-   Copyright (c) 2024 Kevin W. Hamlen            ,,A??=P                 OMMNMZ+
+   Copyright (c) 2025 Kevin W. Hamlen            ,,A??=P                 OMMNMZ+
    The University of Texas at Dallas         =:$ZZ$+ZZI                  7MMZMZ7
    Computer Science Department             Z$$ZM++O++                    7MMZZN+
                                           ZZ$7Z.ZM~?                     7MZDNO$
@@ -16,7 +16,7 @@
    * This module merely defines the core interface       MMMMMMMMMMMMMM7..$MNDM+
      for all simplifiers.  For the code that actually     MMDMMMMMMMMMZ7..$DM$77
      implements simplification, see each simplifier        MMMMMMM+MMMZ7..7ZM~++
-     module (e.g., Picinae_simplifier_v1_0.v).              MMMMMMMMMMM7..ZNOOMZ
+     module (e.g., Picinae_simplifier_v1_1.v).              MMMMMMMMMMM7..ZNOOMZ
                                                              MMMMMMMMMM$.$MOMO=7
                                                               MDMMMMMMMO.7MDM7M+
                                                                ZMMMMMMMM.$MM8$MN
@@ -58,21 +58,15 @@ Require Import Picinae_finterp.
 (* Define tokens to denote each ltac exported by a simplifier. *)
 
 Inductive psimpl_tactic :=
-| PSIMPL_GENN | PSIMPL_GENM | PSIMPL_GENB | PSIMPL_GENS | PSIMPL_GENV | PSIMPL_GENU
+| PSIMPL_GENN | PSIMPL_GENB | PSIMPL_GENS | PSIMPL_GENU
 | PSIMPL_POPULATE_VAR_IDS
 | PSIMPL_N_HYP | PSIMPL_EXHYP_N | PSIMPL_EXGOAL_N
 | PSIMPL_B_HYP | PSIMPL_EXHYP_B | PSIMPL_EXGOAL_B
-| PSIMPL_M_HYP | PSIMPL_EXHYP_M | PSIMPL_EXGOAL_M
 | PSIMPL_S_HYP | PSIMPL_EXHYP_S | PSIMPL_EXGOAL_S
-| PSIMPL_V_HYP | PSIMPL_EXHYP_V | PSIMPL_EXGOAL_V | PSIMPL_V_GOAL
 | PSIMPL_U_HYP | PSIMPL_EXHYP_U | PSIMPL_EXGOAL_U | PSIMPL_U_GOAL.
 
 
-(* Mark all non-nested terms of type N, bool, and addr->N for simplification. *)
-
-Definition _psiN u := match u with VaN n _ => n | _ => N0 end.
-Definition _psiB (b:bool) := b.
-Definition _psiM u := match u with VaM m _ => m | _ => fun _ => 0 end.
+(* Mark all non-nested terms of type N and bool for simplification. *)
 
 Ltac find_containing_term H v A :=
   let v' := fresh A in
@@ -83,34 +77,27 @@ Ltac find_containing_term H v A :=
     rename v' into v
   | subst v' ].
 
+Definition _psimpl_ (A:Type) (x:A) := x.
+
+
+Module Type PSIMPL_BASE (IL: PICINAE_IL).
+
 Ltac psimpl_mark_all_in H :=
   let P := fresh in
   set (P:=_) in (value of H);
   repeat (
-    let u := fresh "u" in
-    set (u:=_:value) in (value of P) at 1;
-    fold u in (value of P);
-    pattern u in (value of P);
-    let Pval := (eval cbv delta [P] in P) in
-    lazymatch Pval with ?f u =>
-      let P' := fresh in
-      set (P' := f) in (value of P);
-      subst u P; rename P' into P
-    end
-  );
-  repeat (
     let e := fresh "e" in
     first [ set (e:=_:N) in (value of P) at 1;
             try find_containing_term P e bool;
-            try find_containing_term P e (addr->N)
+            try find_containing_term P e IL.store
           | set (e:=_:bool) in (value of P) at 1;
-            try find_containing_term P e (addr->N)
-          | set (e:=_:addr->N) in (value of P) at 1 ];
+            try find_containing_term P e IL.store
+          | set (e:=_:IL.store) in (value of P) at 1 ];
     pattern e in (value of P);
-    lazymatch type of e with
-    | N => change e with (_psiN (VaN e 1)) in (value of P)
-    | bool => change e with (_psiB e) in (value of P)
-    | N->addr => change e with (_psiM (VaM e 1)) in (value of P)
+    match type of e with
+    | ?y => unify y N;        change_no_check e with (_psimpl_ N e) in (value of P)
+    | ?y => unify y bool;     change_no_check e with (_psimpl_ bool e) in (value of P)
+    | ?y => unify y IL.store; change_no_check e with (_psimpl_ IL.store e) in (value of P)
     end;
     let Pval := (eval cbv delta [P] in P) in
     lazymatch Pval with ?f _ =>
@@ -126,23 +113,16 @@ Ltac psimpl_mark_all_in H :=
 
 (*** TOP-LEVEL SIMPLIFIER INTERFACE ***)
 
-Module Picinae_Simplifier_Base.
-
 (* Create an initial dummy definition for PSimplifier that will later be replaced
    by one of the real simplifier definitions. *)
 Ltac PSimplifier tac := fail "PSimplifier undefined. Define it with: Ltac PSimplifier ::= PSimplifier_v1_0".
 
 
-(* Syntax 1: psimpl in H.      (* simply all terms of type N, bool, and addr->N in hypothesis H *)
-   Syntax 2: psimpl_vals in H. (* only simplify the terms within IL values (much faster!) *) *)
+(* Syntax 1: psimpl in H.
+   (Simplify all terms of type N, bool, and store in hypothesis H.) *)
 
 Ltac psimpl_vals_hyp H :=
   let t1 := fresh "sast" in
-  (let t := (let Htyp := type of H in PSimplifier PSIMPL_GENV Htyp) in
-   (* idtac "SASTV:" t; *) epose (t1:=t));
-  PSimplifier PSIMPL_V_HYP t1 H;
-  clear t1;
-  PSimplifier PSIMPL_EXHYP_V H;
   (let t0 := fresh "sast" in
    (let t := (let Htyp := type of H in PSimplifier PSIMPL_GENU Htyp) in epose (t0:=t));
    let t0def := (eval cbv delta [t0] in t0) in let t := PSimplifier PSIMPL_POPULATE_VAR_IDS N0 t0def in
@@ -151,7 +131,7 @@ Ltac psimpl_vals_hyp H :=
   clear t1;
   PSimplifier PSIMPL_EXHYP_U H.
 
-Ltac psimpl_all_hyp H :=
+Ltac psimpl_hyp H :=
   let P := fresh in
   set (P:=_) in H;
   psimpl_mark_all_in P;
@@ -164,22 +144,16 @@ Ltac psimpl_all_hyp H :=
       lazymatch type of Heq with _ = ?e => set (H:=e) in Heq end;
       try rewrite Heq in *;
       clear y Heq ];
-  unfold _psiN,_psiB,_psiM in H.
+  unfold _psimpl_ in H.
 
-Tactic Notation "psimpl_vals" "in" hyp(H) := psimpl_vals_hyp H.
-Tactic Notation "psimpl" "in" hyp(H) := psimpl_all_hyp H.
+Tactic Notation "psimpl" "in" hyp(H) := psimpl_hyp H.
 
 
-(* Syntax 1: psimpl.      (* Simplify all exps of type N, bool, and addr->N in the goal. *)
-   Syntax 2: psimpl_vals. (* Only simplify the terms in IL values (much faster!) *) *)
+(* Syntax 2: psimpl.
+   (Simplify all exps of type N, bool, and store in the goal.) *)
 
 Ltac psimpl_vals_goal :=
   let t1 := fresh "sast" in
-  (let t := (lazymatch goal with |- ?g => PSimplifier PSIMPL_GENV g end) in
-   (* idtac "SASTV:" t; *) epose (t1:=t));
-  PSimplifier PSIMPL_V_GOAL t1;
-  clear t1;
-  PSimplifier PSIMPL_EXGOAL_V;
   (let t0 := fresh "sast" in
    (let t := (lazymatch goal with |- ?g => PSimplifier PSIMPL_GENU g end) in epose (t0:=t));
    let t0def := (eval cbv delta [t0] in t0) in let t := PSimplifier PSIMPL_POPULATE_VAR_IDS N0 t0def in
@@ -188,21 +162,21 @@ Ltac psimpl_vals_goal :=
   clear t1;
   PSimplifier PSIMPL_EXGOAL_U.
 
-Ltac psimpl_all_goal :=
+Ltac psimpl_goal :=
   let P := fresh in
   set (P:=_);
   psimpl_mark_all_in P;
   psimpl_vals_goal;
-  unfold _psiN,_psiB,_psiM.
+  unfold _psimpl_.
 
-Tactic Notation "psimpl_vals" := psimpl_vals_goal.
-Tactic Notation "psimpl" := psimpl_all_goal.
+Tactic Notation "psimpl" := psimpl_goal.
 
 
-(* Syntax 1: psimpl e in H.
-   Syntax 2: psimpl e.
-   Description: Simplify subexpression e (must have type N, bool, mem, value, or store)
-   in hypothesis H or in the goal.  Note: e may be a pattern with wildcards (underscores). *)
+(* Syntax 3: psimpl e in H.
+   Syntax 4: psimpl e.
+   (Simplify subexpression e (must have type N, bool, or store)
+   in hypothesis H or in the goal, respectively.
+   Note: e may be a pattern with wildcards (underscores).) *)
 
 Ltac __psimpl_exp_hyp GEN HYP EXHYP x H' :=
   let t1 := fresh "sast" in
@@ -216,9 +190,12 @@ Ltac __psimpl_exp_hyp GEN HYP EXHYP x H' :=
 
 Ltac _psimpl_exp_hyp x H' :=
   lazymatch type of x with
-  | N        => __psimpl_exp_hyp PSIMPL_GENN PSIMPL_N_HYP PSIMPL_EXHYP_N x H'
-  | bool     => __psimpl_exp_hyp PSIMPL_GENB PSIMPL_B_HYP PSIMPL_EXHYP_B x H'
-  | addr->N  => __psimpl_exp_hyp PSIMPL_GENM PSIMPL_M_HYP PSIMPL_EXHYP_M x H'
+  | N         => __psimpl_exp_hyp PSIMPL_GENN PSIMPL_N_HYP PSIMPL_EXHYP_N x H'
+  | addr      => __psimpl_exp_hyp PSIMPL_GENN PSIMPL_N_HYP PSIMPL_EXHYP_N x H'
+  | memory    => __psimpl_exp_hyp PSIMPL_GENN PSIMPL_N_HYP PSIMPL_EXHYP_N x H'
+  | bool      => __psimpl_exp_hyp PSIMPL_GENB PSIMPL_B_HYP PSIMPL_EXHYP_B x H'
+  | IL.store  => __psimpl_exp_hyp PSIMPL_GENS PSIMPL_S_HYP PSIMPL_EXHYP_S x H'
+  | IL.var->N => __psimpl_exp_hyp PSIMPL_GENS PSIMPL_S_HYP PSIMPL_EXHYP_S x H'
   | _ => psimpl_vals_hyp H'
   end.
 
@@ -243,4 +220,9 @@ Ltac psimpl_exp_goal e :=
 Tactic Notation "psimpl" uconstr(e) "in" hyp(H) := psimpl_exp_hyp uconstr:(e) H.
 Tactic Notation "psimpl" uconstr(e) := psimpl_exp_goal uconstr:(e).
 
+End PSIMPL_BASE.
+
+
+Module Picinae_Simplifier_Base (IL: PICINAE_IL) : PSIMPL_BASE IL.
+  Include PSIMPL_BASE IL.
 End Picinae_Simplifier_Base.
